attempt one: adding invId: forall T, TFun T T.
This does not pass the progress theorem, as the following case was not dismissed

jt_term Delta (TDefault T0 :: Gamma_cl) t_cl (TDefault T0)
---
exists s2 : state, cred (mode_cont (CClosure t_cl sigma_cl :: kappa) env REmpty) s2.

theories/typing.v
@@ -62,6 +62,9 @@ Inductive inv_root: type -> Prop :=
     forall T,
       inv_thunked_or_nodefault T ->
       inv_root T
+  | invId:
+    forall T,
+      inv_root (TFun T T)
 .
 
 
@@ -107,9 +110,9 @@ Module Invariant_Examples.
 
   Example negative_1: not (inv_root (TDefault (TDefault TInteger))). intro. repeat sinv_inv. Qed.
   Example negative_2: not (inv_root (TDefault (TFun TBool (TDefault TInteger)))). intro. repeat sinv_inv. Qed.
-  Example negative_3: not (inv_root (TFun (TDefault TBool) TInteger)). intro. repeat sinv_inv. Qed.
+  Example negative_3: not (inv_root (TFun (TDefault TBool) TInteger)). intro. repeat sinv_inv; inj. Qed.
   Example negative_4: not (inv_root (TFun (TFun TInteger (TDefault TBool)) (TDefault TBool))).
-  intro. repeat sinv_inv. Qed.
+  intro. repeat sinv_inv; inj. Qed.
 
 End Invariant_Examples.
 
@@ -512,19 +515,16 @@ In
 
   ) (TFun (TFun TUnit (TDefault TInteger)) TInteger).
   Proof.
-    Ltac finish:= simpl; eauto; try solve [repeat econs_inv | eapply invThunkedOrNoDefault; repeat econs_inv].
+    Ltac finish:= simpl; eauto; try solve [repeat econs_inv | eapply invThunkedOrNoDefault; repeat econs_inv|eapply invId].
     repeat econs_jt; finish.
-    { repeat econs_inv; admit. }
-    { repeat econs_inv; admit. }
-    { repeat econs_inv; admit. }
-  Admitted.
+  Qed.
 
   (* (λ t. < t () | true :- pure 5>) (λ x. Ø) *)
   Example negative_1: ~ jt_term (fun _ => None) [] (App (Lam ((Default [App (Var 0) (Value (VUnit))] (Value (Bool true)) (DefaultPure (Value (Int 5)))))) (Lam Empty)) (TDefault TInteger).
     intro.
     repeat sinv_jt.
     clear -H10.
-    repeat sinv_inv.
+    repeat sinv_inv; inj.
   Qed.
 End Typing_Examples.
 
